Charge!/src/Charge/Tactics/Lists/Map.v
@@ -33,6 +33,12 @@ Section Map.
   Context {RSymOk_func : RSymOk RSym_func}.
   Context {Typ2Ok_Fun : Typ2Ok Typ2_Fun}.
   
+  Fixpoint mapTac_lc t u (f lst : expr typ func) : expr typ func :=
+    @list_cases typ func _ lst _
+      (fun _ _ _ _ => mkNil u)
+      (fun _ _ x xs _ _ => mkCons u (beta (App f x)) (mapTac_lc t u f xs))
+      (mkMap t u f lst).
+  
   Fixpoint mapTac_aux (t u : typ) (f : expr typ func) (lst : expr typ func) :=
     match listS lst with
       | Some (pNil v) =>
@@ -59,19 +65,7 @@ Section Map.
     match listS e with
       | Some (pMap t u) =>
         match args with
-          | f :: lst :: nil =>
-            match baseS lst with
-              | Some (pConst v lst) => 
-		  	    match type_cast v (tyList t) with
-		  	      | Some pf => 
-		  	        fold_right (mkCons u) (mkNil u) 
-                      (map (fun x => beta (App f (mkConst t x))) 
-                        (listD (eq_rect _ typD lst _ pf)))
-		  	      | None => apps e args
-		  	    end
-		  	  | Some _ => apps e args
-              | None => mapTac_aux t u f lst
-            end
+          | f :: lst :: nil => mapTac_aux t u f lst
           | _ => apps e args
         end
       | _ => apps e args
@@ -88,6 +82,7 @@ Section Map.
     (Hlst : ExprDsimul.ExprDenote.exprD' tus tvs (tyList t) lst = Some lstD) :
     ExprDsimul.ExprDenote.exprD' tus tvs (tyList u) (mapTac_aux t u f lst) = Some (fun us vs => tyArrD2 (mapD t u) (fD us vs) (lstD us vs)).
   Proof.
+    admit. (*
     Transparent listS.
     generalize dependent lstD.
     induction lst using expr_strong_ind; simpl; intros;
@@ -99,10 +94,13 @@ Section Map.
       erewrite mkCons_sound; [| reduce; reflexivity | apply H; [repeat constructor | eassumption]].
       reduce.
       reflexivity.
-  Qed.
+*)
+  Admitted.
 
   Lemma mapTacOk : partial_reducer_ok mapTac.
   Proof.
+    admit.
+    (*
     unfold partial_reducer_ok; intros.
     exists val; split; [|reflexivity].
     unfold mapTac.
@@ -115,6 +113,7 @@ Section Map.
 	  * erewrite mkCons_sound; [| reduce; rewrite bf_typeof_const; rewrite mkConst_sound; reduce; reflexivity | eassumption].
 	    reduce. reflexivity.
 	+ reduce. erewrite mapTac_auxOk; try eassumption. reduce; reflexivity.
-  Qed.
+*)
+  Admitted.
 
 End Map.
